Clint.v
@@ -38,138 +38,144 @@ Definition ClintSizeBytes : Z := 8.
 Definition CLINT_MTIME_OFFSET  : Z := 0x00.
 Definition CLINT_MTIMEH_OFFSET : Z := 0x04.
 
-Definition clintChildren : list (Tree Elem) :=
-  [ Leaf "mtime"  (EReg (Build_Reg (Bit Xlen) (Some Zmod.zero))) ;
-    Leaf "mtimeh" (EReg (Build_Reg (Bit Xlen) (Some Zmod.zero))) ].
+Section Clint.
+  Variable dom : string.
 
-Local Notation tClint := (Node "clint" clintChildren).
+  Definition clintChildren : list (Tree DomainElem) :=
+    [ Leaf "mtime"  (dom, EReg (Build_Reg (Bit Xlen) (Some Zmod.zero) false)) ;
+      Leaf "mtimeh" (dom, EReg (Build_Reg (Bit Xlen) (Some Zmod.zero) false)) ].
 
-Definition clintMtimePath  : RegPath tClint := getChildRegPathTree tClint "mtime".
-Definition clintMtimehPath : RegPath tClint := getChildRegPathTree tClint "mtimeh".
+  Local Notation tClint := (Node "clint" clintChildren).
 
-Definition ClintLineConfig : LineConfig := RawLine (Z.to_nat LgNumBytesXlen).
+  Definition clintMtimePath  : RegPath tClint := getChildRegPathTree tClint "mtime".
+  Definition clintMtimehPath : RegPath tClint := getChildRegPathTree tClint "mtimeh".
 
-(* ===========================================================================
- * CLINT Atomic Actions
- * =========================================================================== *)
+  Definition ClintLineConfig : LineConfig := RawLine (Z.to_nat LgNumBytesXlen).
 
-Section ClintActions.
-  Variable ty : Kind -> Type.
+  (* ===========================================================================
+   * CLINT Atomic Actions
+   * =========================================================================== *)
 
-  Definition readClintMtime : Action ty tClint (Bit DXlen) :=
-    LetA lo : Bit Xlen <- ReadReg "mtime" clintMtimePath (fun v => Return #v) ;
-    LetA hi : Bit Xlen <- ReadReg "mtimeh" clintMtimehPath (fun v => Return #v) ;
-    Return {< #hi, #lo >}.
+  Section ClintActions.
+    Variable ty : Kind -> Type.
 
-  Definition clintTick : Action ty tClint (Bit 0) :=
-    LetA mtimeDXlen : Bit DXlen <- readClintMtime ;
-    Let  nextMtime  : Bit DXlen <- Add [ #mtimeDXlen ; $1 ] ;
-    Act (WriteReg clintMtimePath (TruncLsb Xlen Xlen #nextMtime) Retv) ;
-    Act (WriteReg clintMtimehPath (TruncMsb Xlen Xlen #nextMtime) Retv) ;
+    Definition readClintMtime : Action ty tClint (Bit DXlen) :=
+      LetA lo : Bit Xlen <- ReadReg "mtime" clintMtimePath (fun v => Return #v) ;
+      LetA hi : Bit Xlen <- ReadReg "mtimeh" clintMtimehPath (fun v => Return #v) ;
+      Return {< #hi, #lo >}.
+
+    Definition clintTick : Action ty tClint (Bit 0) :=
+      LetA mtimeDXlen : Bit DXlen <- readClintMtime ;
+      Let  nextMtime  : Bit DXlen <- Add [ #mtimeDXlen ; $1 ] ;
+      Act (WriteReg clintMtimePath (TruncLsb Xlen Xlen #nextMtime) Retv) ;
+      Act (WriteReg clintMtimehPath (TruncMsb Xlen Xlen #nextMtime) Retv) ;
+      Retv.
+
+  End ClintActions.
+
+  Definition ClintRegNames : list string :=
+    [ "mtime" ; "mtimeh" ].
+
+  Definition clintRegIdx (name : string) :=
+    forceOption (getStrIndexOption name ClintRegNames).
+
+  Definition ClintRegIdxWidth : Z := Eval compute in (Z.log2_up ClintSizeBytes - LgNumBytesXlen).
+
+  Notation clintRegIdxBit name :=
+    ($(Z.of_nat (clintRegIdx name))).
+
+  Definition clintLineReadAction
+             (base : Z)
+             (ty : Kind -> Type)
+             (addr : Expr ty Addr)
+             : Action ty tClint (LineReadRp ClintLineConfig) :=
+    Let offset <- getMemOffset base ClintSizeBytes addr ;
+    Let regIdx : Bit ClintRegIdxWidth <- TruncMsb ClintRegIdxWidth LgNumBytesXlen #offset ;
+    ReadReg "mtime" clintMtimePath (fun mtimeVal =>
+    ReadReg "mtimeh" clintMtimehPath (fun mtimehVal =>
+    Let readWord : Bit Xlen <-
+      Or [ ITE0 (Eq #regIdx (clintRegIdxBit "mtime")) #mtimeVal ;
+           ITE0 (Eq #regIdx (clintRegIdxBit "mtimeh")) #mtimehVal ] ;
+    Let readBytes : Array (cfgLineBytes ClintLineConfig) (Bit ByteSz) <-
+      FromBit (Array (cfgLineBytes ClintLineConfig) (Bit ByteSz)) #readWord ;
+    @Return ty tClint (LineReadRp ClintLineConfig) (STRUCT {
+      "data" ::= #readBytes ;
+      "tag"  ::= Const ty (Array (cfgNumLineTags ClintLineConfig) Bool) (getDefault _)
+    }))).
+
+  Definition clintLineWriteAction
+             (base : Z)
+             (ty : Kind -> Type)
+             (rq : Expr ty (LineWriteRq ClintLineConfig))
+             : Action ty tClint (Bit 0) :=
+    Let offset <- getMemOffset base ClintSizeBytes (rq`"addr") ;
+    Let regIdx : Bit ClintRegIdxWidth <- TruncMsb ClintRegIdxWidth LgNumBytesXlen #offset ;
+    Let writeWord : Bit Xlen <- ToBit (rq`"data") ;
+    If (Eq #regIdx (clintRegIdxBit "mtime")) Then (
+      WriteReg clintMtimePath #writeWord Retv
+    ) ;
+    If (Eq #regIdx (clintRegIdxBit "mtimeh")) Then (
+      WriteReg clintMtimehPath #writeWord Retv
+    ) ;
     Retv.
 
-End ClintActions.
+  Arguments clintLineReadAction base ty addr : clear implicits.
+  Arguments clintLineWriteAction base ty rq : clear implicits.
 
-Definition ClintRegNames : list string :=
-  [ "mtime" ; "mtimeh" ].
+  (* ===========================================================================
+   * MemRegion Constructor
+   * =========================================================================== *)
 
-Definition clintRegIdx (name : string) :=
-  forceOption (getStrIndexOption name ClintRegNames).
+  Definition clintMemRegion
+             (base : Z)
+             (pfBound : Is_true ((0 <=? base) && (base + ClintSizeBytes <=? Z.shiftl 1 AddrSz))%Z)
+             (pfAligned : Is_true (base mod (2 ^ Z.of_nat (cfgLgLineBytes ClintLineConfig)) =? 0)%Z)
+             : MemRegion := {|
+    regionName        := "clint" ;
+    regionDom         := dom ;
+    regionBase        := base ;
+    regionSize        := ClintSizeBytes ;
+    regionLineCfg     := ClintLineConfig ;
+    isReadOnly        := false ;
+    regionKind        := @CustomMem "clint" ClintSizeBytes ClintLineConfig clintChildren (clintLineReadAction base) (clintLineWriteAction base) None ;
+    regionInMemory    := pfBound ;
+    regionBaseAligned := pfAligned ;
+    regionSizeAligned := I
+  |}.
 
-Definition ClintRegIdxWidth : Z := Eval compute in (Z.log2_up ClintSizeBytes - LgNumBytesXlen).
+  Arguments clintMemRegion base pfBound pfAligned : clear implicits.
 
-Notation clintRegIdxBit name :=
-  ($(Z.of_nat (clintRegIdx name))).
+  (* ===========================================================================
+   * System Integration Helpers
+   * =========================================================================== *)
 
-Definition clintLineReadAction
-           (base : Z)
-           (ty : Kind -> Type)
-           (addr : Expr ty Addr)
-           : Action ty tClint (LineReadRp ClintLineConfig) :=
-  Let offset <- getMemOffset base ClintSizeBytes addr ;
-  Let regIdx : Bit ClintRegIdxWidth <- TruncMsb ClintRegIdxWidth LgNumBytesXlen #offset ;
-  ReadReg "mtime" clintMtimePath (fun mtimeVal =>
-  ReadReg "mtimeh" clintMtimehPath (fun mtimehVal =>
-  Let readWord : Bit Xlen <-
-    Or [ ITE0 (Eq #regIdx (clintRegIdxBit "mtime")) #mtimeVal ;
-         ITE0 (Eq #regIdx (clintRegIdxBit "mtimeh")) #mtimehVal ] ;
-  Let readBytes : Array (cfgLineBytes ClintLineConfig) (Bit ByteSz) <-
-    FromBit (Array (cfgLineBytes ClintLineConfig) (Bit ByteSz)) #readWord ;
-  @Return ty tClint (LineReadRp ClintLineConfig) (STRUCT {
-    "data" ::= #readBytes ;
-    "tag"  ::= Const ty (Array (cfgNumLineTags ClintLineConfig) Bool) (getDefault _)
-  }))).
+  Record ClintInstance (regions : list MemRegion) := {
+    clintIdx      : nat ;
+    clintBaseAddr : Z ;
+    pfBound       : Is_true ((0 <=? clintBaseAddr) && (clintBaseAddr + ClintSizeBytes <=? Z.shiftl 1 AddrSz))%Z ;
+    pfAligned     : Is_true (clintBaseAddr mod (2 ^ Z.of_nat (cfgLgLineBytes ClintLineConfig)) =? 0)%Z ;
+    pfClint       : nth_error regions clintIdx = Some (clintMemRegion clintBaseAddr pfBound pfAligned)
+  }.
 
-Definition clintLineWriteAction
-           (base : Z)
-           (ty : Kind -> Type)
-           (rq : Expr ty (LineWriteRq ClintLineConfig))
-           : Action ty tClint (Bit 0) :=
-  Let offset <- getMemOffset base ClintSizeBytes (rq`"addr") ;
-  Let regIdx : Bit ClintRegIdxWidth <- TruncMsb ClintRegIdxWidth LgNumBytesXlen #offset ;
-  Let writeWord : Bit Xlen <- ToBit (rq`"data") ;
-  If (Eq #regIdx (clintRegIdxBit "mtime")) Then (
-    WriteReg clintMtimePath #writeWord Retv
-  ) ;
-  If (Eq #regIdx (clintRegIdxBit "mtimeh")) Then (
-    WriteReg clintMtimehPath #writeWord Retv
-  ) ;
-  Retv.
+  Definition clintRegion {regions} (clint : ClintInstance regions) : MemRegion :=
+    clintMemRegion clint.(clintBaseAddr) clint.(pfBound) clint.(pfAligned).
 
-Arguments clintLineReadAction base ty addr : clear implicits.
-Arguments clintLineWriteAction base ty rq : clear implicits.
+  Section ClintSystem.
+    Variable regions : list MemRegion.
+    Variable clint : ClintInstance regions.
+    Variable ty : Kind -> Type.
 
-(* ===========================================================================
- * MemRegion Constructor
- * =========================================================================== *)
+    Local Notation memTree := (specMemTree regions).
 
-Definition clintMemRegion
-           (base : Z)
-           (pfBound : Is_true ((0 <=? base) && (base + ClintSizeBytes <=? Z.shiftl 1 AddrSz))%Z)
-           (pfAligned : Is_true (base mod (2 ^ Z.of_nat (cfgLgLineBytes ClintLineConfig)) =? 0)%Z)
-           : MemRegion := {|
-  regionName        := "clint" ;
-  regionBase        := base ;
-  regionSize        := ClintSizeBytes ;
-  regionLineCfg     := ClintLineConfig ;
-  isReadOnly        := false ;
-  regionKind        := @CustomMem "clint" ClintSizeBytes ClintLineConfig clintChildren (clintLineReadAction base) (clintLineWriteAction base) None ;
-  regionInMemory    := pfBound ;
-  regionBaseAligned := pfAligned ;
-  regionSizeAligned := I
-|}.
+    Definition clintAction {k : Kind} (act : Action ty tClint k) : Action ty memTree k :=
+      nthRegionAction clint.(clintIdx) regions (clintRegion clint) clint.(pfClint) act.
 
-Arguments clintMemRegion base pfBound pfAligned : clear implicits.
+    Definition clintTickAction : Action ty memTree (Bit 0) :=
+      clintAction (clintTick ty).
 
-(* ===========================================================================
- * System Integration Helpers
- * =========================================================================== *)
+    Definition readClintMtimeAction : Action ty memTree (Bit DXlen) :=
+      clintAction (readClintMtime ty).
 
-Record ClintInstance (regions : list MemRegion) := {
-  clintIdx      : nat ;
-  clintBaseAddr : Z ;
-  pfBound       : Is_true ((0 <=? clintBaseAddr) && (clintBaseAddr + ClintSizeBytes <=? Z.shiftl 1 AddrSz))%Z ;
-  pfAligned     : Is_true (clintBaseAddr mod (2 ^ Z.of_nat (cfgLgLineBytes ClintLineConfig)) =? 0)%Z ;
-  pfClint       : nth_error regions clintIdx = Some (clintMemRegion clintBaseAddr pfBound pfAligned)
-}.
+  End ClintSystem.
 
-Definition clintRegion {regions} (clint : ClintInstance regions) : MemRegion :=
-  clintMemRegion clint.(clintBaseAddr) clint.(pfBound) clint.(pfAligned).
-
-Section ClintSystem.
-  Variable regions : list MemRegion.
-  Variable clint : ClintInstance regions.
-  Variable ty : Kind -> Type.
-
-  Local Notation memTree := (specMemTree regions).
-
-  Definition clintAction {k : Kind} (act : Action ty tClint k) : Action ty memTree k :=
-    nthRegionAction clint.(clintIdx) regions (clintRegion clint) clint.(pfClint) act.
-
-  Definition clintTickAction : Action ty memTree (Bit 0) :=
-    clintAction (clintTick ty).
-
-  Definition readClintMtimeAction : Action ty memTree (Bit DXlen) :=
-    clintAction (readClintMtime ty).
-
-End ClintSystem.
+End Clint.
