SifiveUartController.v
@@ -62,368 +62,382 @@ Definition SifiveUartFifoCountWidth : Z :=
   Eval compute in (Z.log2_up (Z.of_nat (SifiveUartFifoCapacity + 1))).
 
 (* Helper to read size/count from a fifoTree *)
-Definition fifoCount {capacity : nat} {k : Kind} {ty : Kind -> Type} :
-  Action ty (fifoTree capacity k) (Bit (Z.log2_up (Z.of_nat (capacity + 1)))) :=
-  RegRead sz <- "fifo.size" in (fifoTree capacity k) ;
+Definition fifoCount {dom : string} {capacity : nat} {k : Kind} {ty : Kind -> Type} :
+  Action ty (fifoTree dom capacity k) (Bit (Z.log2_up (Z.of_nat (capacity + 1)))) :=
+  RegRead sz <- "fifo.size" in (fifoTree dom capacity k) ;
   Return #sz.
 
 (* ===========================================================================
  * SiFive UART Tree Definition
  * =========================================================================== *)
 
-Definition sifiveUartChildren : list (Tree Elem) :=
-  [ Node "tx" [ fifoTree SifiveUartFifoCapacity (Bit 8) ] ;
-    Node "rx" [ fifoTree SifiveUartFifoCapacity (Bit 8) ] ;
-    Leaf "txctrl_txen"  (EReg (Build_Reg Bool (Some false))) ;
-    Leaf "txctrl_nstop" (EReg (Build_Reg Bool (Some false))) ;
-    Leaf "txctrl_txcnt" (EReg (Build_Reg (Bit SifiveUartWatermarkWidth) (Some Zmod.zero))) ;
-    Leaf "rxctrl_rxen"  (EReg (Build_Reg Bool (Some false))) ;
-    Leaf "rxctrl_rxcnt" (EReg (Build_Reg (Bit SifiveUartWatermarkWidth) (Some Zmod.zero))) ;
-    Leaf "ie_txwm"      (EReg (Build_Reg Bool (Some false))) ;
-    Leaf "ie_rxwm"      (EReg (Build_Reg Bool (Some false))) ;
-    Leaf "ip_txwm"      (EReg (Build_Reg Bool (Some false))) ;
-    Leaf "ip_rxwm"      (EReg (Build_Reg Bool (Some false))) ;
-    Leaf "div"          (EReg (Build_Reg (Bit 16) (Some Zmod.zero))) ;
-    Leaf "txData"       (ESend (Bit 8)) ;
-    Leaf "txRdy"        (ERecv Bool) ;
-    Leaf "rxData"       (ERecv (Option (Bit 8))) ;
-    Leaf "rxRdy"        (ESend (Bit 0)) ;
-    Leaf "divOut"       (ESend (Bit 16))
-  ].
+Section SifiveUart.
+  Variable dom : string.
 
-Definition sifiveUartTree : Tree Elem :=
-  Node "sifive_uart" sifiveUartChildren.
+  Definition sifiveUartChildren : list (Tree DomainElem) :=
+    [ Node "tx" [ fifoTree dom SifiveUartFifoCapacity (Bit 8) ] ;
+      Node "rx" [ fifoTree dom SifiveUartFifoCapacity (Bit 8) ] ;
+      Leaf "txctrl_txen"  (dom, EReg (Build_Reg Bool (Some false) false)) ;
+      Leaf "txctrl_nstop" (dom, EReg (Build_Reg Bool (Some false) false)) ;
+      Leaf "txctrl_txcnt" (dom, EReg (Build_Reg (Bit SifiveUartWatermarkWidth) (Some Zmod.zero) false)) ;
+      Leaf "rxctrl_rxen"  (dom, EReg (Build_Reg Bool (Some false) false)) ;
+      Leaf "rxctrl_rxcnt" (dom, EReg (Build_Reg (Bit SifiveUartWatermarkWidth) (Some Zmod.zero) false)) ;
+      Leaf "ie_txwm"      (dom, EReg (Build_Reg Bool (Some false) false)) ;
+      Leaf "ie_rxwm"      (dom, EReg (Build_Reg Bool (Some false) false)) ;
+      Leaf "ip_txwm"      (dom, EReg (Build_Reg Bool (Some false) false)) ;
+      Leaf "ip_rxwm"      (dom, EReg (Build_Reg Bool (Some false) false)) ;
+      Leaf "irq"          (dom, EReg (Build_Reg Bool (Some false) true)) ;
+      Leaf "div"          (dom, EReg (Build_Reg (Bit 16) (Some Zmod.zero) false)) ;
+      Leaf "txData"       (dom, ESend (Bit 8)) ;
+      Leaf "txRdy"        (dom, ERecv Bool) ;
+      Leaf "rxData"       (dom, ERecv (Option (Bit 8))) ;
+      Leaf "rxRdy"        (dom, ESend (Bit 0)) ;
+      Leaf "divOut"       (dom, ESend (Bit 16))
+    ].
 
-Definition SifiveUartLineConfig : LineConfig := RawLine (Z.to_nat LgNumBytesXlen).
+  Definition sifiveUartTree : Tree DomainElem :=
+    Node "sifive_uart" sifiveUartChildren.
 
-(* ===========================================================================
- * Paths & Embeddings
- * =========================================================================== *)
+  Definition SifiveUartLineConfig : LineConfig := RawLine (Z.to_nat LgNumBytesXlen).
 
-Definition sifiveUartTxctrlTxenPath  : RegPath sifiveUartTree := getChildRegPathTree sifiveUartTree "txctrl_txen".
-Definition sifiveUartTxctrlNstopPath : RegPath sifiveUartTree := getChildRegPathTree sifiveUartTree "txctrl_nstop".
-Definition sifiveUartTxctrlTxcntPath : RegPath sifiveUartTree := getChildRegPathTree sifiveUartTree "txctrl_txcnt".
+  (* ===========================================================================
+   * Paths & Embeddings
+   * =========================================================================== *)
 
-Definition sifiveUartRxctrlRxenPath  : RegPath sifiveUartTree := getChildRegPathTree sifiveUartTree "rxctrl_rxen".
-Definition sifiveUartRxctrlRxcntPath : RegPath sifiveUartTree := getChildRegPathTree sifiveUartTree "rxctrl_rxcnt".
+  Definition sifiveUartTxctrlTxenPath  : RegPath sifiveUartTree := getChildRegPathTree sifiveUartTree "txctrl_txen".
+  Definition sifiveUartTxctrlNstopPath : RegPath sifiveUartTree := getChildRegPathTree sifiveUartTree "txctrl_nstop".
+  Definition sifiveUartTxctrlTxcntPath : RegPath sifiveUartTree := getChildRegPathTree sifiveUartTree "txctrl_txcnt".
 
-Definition sifiveUartIeTxwmPath      : RegPath sifiveUartTree := getChildRegPathTree sifiveUartTree "ie_txwm".
-Definition sifiveUartIeRxwmPath      : RegPath sifiveUartTree := getChildRegPathTree sifiveUartTree "ie_rxwm".
+  Definition sifiveUartRxctrlRxenPath  : RegPath sifiveUartTree := getChildRegPathTree sifiveUartTree "rxctrl_rxen".
+  Definition sifiveUartRxctrlRxcntPath : RegPath sifiveUartTree := getChildRegPathTree sifiveUartTree "rxctrl_rxcnt".
 
-Definition sifiveUartIpTxwmPath      : RegPath sifiveUartTree := getChildRegPathTree sifiveUartTree "ip_txwm".
-Definition sifiveUartIpRxwmPath      : RegPath sifiveUartTree := getChildRegPathTree sifiveUartTree "ip_rxwm".
+  Definition sifiveUartIeTxwmPath      : RegPath sifiveUartTree := getChildRegPathTree sifiveUartTree "ie_txwm".
+  Definition sifiveUartIeRxwmPath      : RegPath sifiveUartTree := getChildRegPathTree sifiveUartTree "ie_rxwm".
 
-Definition sifiveUartDivPath         : RegPath sifiveUartTree := getChildRegPathTree sifiveUartTree "div".
+  Definition sifiveUartIpTxwmPath      : RegPath sifiveUartTree := getChildRegPathTree sifiveUartTree "ip_txwm".
+  Definition sifiveUartIpRxwmPath      : RegPath sifiveUartTree := getChildRegPathTree sifiveUartTree "ip_rxwm".
 
-Definition sifiveUartTxDataPath      : SendPath sifiveUartTree := getChildSendPathTree sifiveUartTree "txData".
-Definition sifiveUartTxRdyPath       : RecvPath sifiveUartTree := getChildRecvPathTree sifiveUartTree "txRdy".
-Definition sifiveUartRxDataPath      : RecvPath sifiveUartTree := getChildRecvPathTree sifiveUartTree "rxData".
-Definition sifiveUartRxRdyPath       : SendPath sifiveUartTree := getChildSendPathTree sifiveUartTree "rxRdy".
-Definition sifiveUartDivOutPath      : SendPath sifiveUartTree := getChildSendPathTree sifiveUartTree "divOut".
+  Definition sifiveUartIrqPath         : RegPath sifiveUartTree := getChildRegPathTree sifiveUartTree "irq".
 
-Definition np_tx_fifo : NodePath sifiveUartTree :=
-  getNodePath sifiveUartTree "sifive_uart.tx.fifo".
+  Definition sifiveUartDivPath         : RegPath sifiveUartTree := getChildRegPathTree sifiveUartTree "div".
 
-Definition np_rx_fifo : NodePath sifiveUartTree :=
-  getNodePath sifiveUartTree "sifive_uart.rx.fifo".
+  Definition sifiveUartTxDataPath      : SendPath sifiveUartTree := getChildSendPathTree sifiveUartTree "txData".
+  Definition sifiveUartTxRdyPath       : RecvPath sifiveUartTree := getChildRecvPathTree sifiveUartTree "txRdy".
+  Definition sifiveUartRxDataPath      : RecvPath sifiveUartTree := getChildRecvPathTree sifiveUartTree "rxData".
+  Definition sifiveUartRxRdyPath       : SendPath sifiveUartTree := getChildSendPathTree sifiveUartTree "rxRdy".
+  Definition sifiveUartDivOutPath      : SendPath sifiveUartTree := getChildSendPathTree sifiveUartTree "divOut".
 
-(* Helper to lift an action across equality of tree nodes *)
-Definition liftActionEq {ty : Kind -> Type} {t : Tree Elem} {k : Kind}
-  (p : NodePath t) {t' : Tree Elem} (H : getNode p = t') (a : Action ty t' k) : Action ty t k :=
-  match H in _ = X return Action ty X k -> Action ty t k with
-  | eq_refl => liftAction (ty:=ty) p (k:=k)
-  end a.
-Arguments liftActionEq [ty t k] p [t'] H a.
+  Definition np_tx_fifo : NodePath sifiveUartTree :=
+    getNodePath sifiveUartTree "sifive_uart.tx.fifo".
 
-(* ===========================================================================
- * SiFive UART Internal Operations
- * =========================================================================== *)
+  Definition np_rx_fifo : NodePath sifiveUartTree :=
+    getNodePath sifiveUartTree "sifive_uart.rx.fifo".
 
-Section SifiveUartOperations.
-  Variable ty : Kind -> Type.
+  (* Helper to lift an action across equality of tree nodes *)
+  Definition liftActionEq {ty : Kind -> Type} {t : Tree DomainElem} {k : Kind}
+    (p : NodePath t) {t' : Tree DomainElem} (H : getNode p = t') (a : Action ty t' k) : Action ty t k :=
+    match H in _ = X return Action ty X k -> Action ty t k with
+    | eq_refl => liftAction (ty:=ty) p (k:=k)
+    end a.
+  Arguments liftActionEq [ty t k] p [t'] H a.
 
-  (* Read txdata: bit 31 indicates whether TX FIFO is full *)
-  Definition readTxData : Action ty sifiveUartTree (Bit Xlen) :=
-    LetA txFull : Bool <- liftAction np_tx_fifo (@isFull SifiveUartFifoCapacity (Bit 8) ty) ;
-    Return {< ToBit #txFull, Const ty (Bit (Xlen - 1)) Zmod.zero >}.
+  (* ===========================================================================
+   * SiFive UART Internal Operations
+   * =========================================================================== *)
 
-  (* Read rxdata: dequeues byte from RX FIFO if available, bit 31 indicates empty *)
-  Definition readRxData : Action ty sifiveUartTree (Bit Xlen) :=
-    LetA rxEmpty : Bool <- liftAction np_rx_fifo (@isEmpty SifiveUartFifoCapacity (Bit 8) ty) ;
-    LetIf rxByte : Bit 8 <-
-      If (Not #rxEmpty) Then (
-        LetA rxHead : Option (Bit 8) <- liftAction np_rx_fifo (@first SifiveUartFifoCapacity (Bit 8) ty) ;
-        Act (liftAction np_rx_fifo (@deq SifiveUartFifoCapacity (Bit 8) ty)) ;
-        Return (##rxHead `! "Some")
-      ) Else (
-        Return $0
-      ) ;
-    Return {< ToBit #rxEmpty, Const ty (Bit (Xlen - 9)) Zmod.zero, #rxByte >}.
+  Section SifiveUartOperations.
+    Variable ty : Kind -> Type.
 
-  (* Read ip: reads registered interrupt pending flags *)
-  Definition readIp : Action ty sifiveUartTree (Bit Xlen) :=
-    LetA txwm_ip : Bool <- ReadReg "ip_txwm" sifiveUartIpTxwmPath (fun v => Return #v) ;
-    LetA rxwm_ip : Bool <- ReadReg "ip_rxwm" sifiveUartIpRxwmPath (fun v => Return #v) ;
-    Return {< Const ty (Bit (Xlen - 2)) Zmod.zero, ToBit #rxwm_ip, ToBit #txwm_ip >}.
+    (* Read txdata: bit 31 indicates whether TX FIFO is full *)
+    Definition readTxData : Action ty sifiveUartTree (Bit Xlen) :=
+      LetA txFull : Bool <- liftAction np_tx_fifo (@isFull dom SifiveUartFifoCapacity (Bit 8) ty) ;
+      Return {< ToBit #txFull, Const ty (Bit (Xlen - 1)) Zmod.zero >}.
 
-  (* Autonomous rule to update ip_txwm and ip_rxwm registers *)
-  Definition sifiveUartIpStep : Action ty sifiveUartTree (Bit 0) :=
-    LetA txCount : Bit SifiveUartFifoCountWidth <- liftAction np_tx_fifo (@fifoCount SifiveUartFifoCapacity (Bit 8) ty) ;
-    LetA rxCount : Bit SifiveUartFifoCountWidth <- liftAction np_rx_fifo (@fifoCount SifiveUartFifoCapacity (Bit 8) ty) ;
-    LetA txcnt   : Bit SifiveUartWatermarkWidth <- ReadReg "txctrl_txcnt" sifiveUartTxctrlTxcntPath (fun v => Return #v) ;
-    LetA rxcnt   : Bit SifiveUartWatermarkWidth <- ReadReg "rxctrl_rxcnt" sifiveUartRxctrlRxcntPath (fun v => Return #v) ;
-    Let txwm_ip  : Bool <- Slt #txCount (ZeroExtendTo SifiveUartFifoCountWidth #txcnt) ;
-    Let rxwm_ip  : Bool <- Sgt #rxCount (ZeroExtendTo SifiveUartFifoCountWidth #rxcnt) ;
-    Act (WriteReg sifiveUartIpTxwmPath #txwm_ip Retv) ;
-    WriteReg sifiveUartIpRxwmPath #rxwm_ip Retv.
-
-  (* SiFive UART Interrupt Output: evaluated for PLIC connection *)
-  Definition sifiveUartIrq : Action ty sifiveUartTree Bool :=
-    LetA txwm_ip : Bool <- ReadReg "ip_txwm" sifiveUartIpTxwmPath (fun v => Return #v) ;
-    LetA rxwm_ip : Bool <- ReadReg "ip_rxwm" sifiveUartIpRxwmPath (fun v => Return #v) ;
-    LetA ie_txwm : Bool <- ReadReg "ie_txwm" sifiveUartIeTxwmPath (fun v => Return #v) ;
-    LetA ie_rxwm : Bool <- ReadReg "ie_rxwm" sifiveUartIeRxwmPath (fun v => Return #v) ;
-    Let tx_irq   : Bool <- And [ #txwm_ip ; #ie_txwm ] ;
-    Let rx_irq   : Bool <- And [ #rxwm_ip ; #ie_rxwm ] ;
-    Let any_irq  : Bool <- Or [ #tx_irq ; #rx_irq ] ;
-    Return #any_irq.
-
-  (* =========================================================================
-   * Decoupled Hardware Rules for Streaming PHY Interface & Divisor Export
-   * ========================================================================= *)
-
-  (* Autonomous rule to export divisor on divOut *)
-  Definition sifiveUartDivStep : Action ty sifiveUartTree (Bit 0) :=
-    ReadReg "div" sifiveUartDivPath (fun divVal =>
-      Send sifiveUartDivOutPath #divVal Retv
-    ).
-
-  (* TX Rule: When enabled and not empty, presents data on txData and dequeues on txRdy *)
-  Definition sifiveUartTxStep : Action ty sifiveUartTree (Bit 0) :=
-    LetA txen : Bool <- ReadReg "txctrl_txen" sifiveUartTxctrlTxenPath (fun v => Return #v) ;
-    If #txen Then (
-      LetA txEmpty : Bool <- liftAction np_tx_fifo (@isEmpty SifiveUartFifoCapacity (Bit 8) ty) ;
-      If (Not #txEmpty) Then (
-        LetA txHead : Option (Bit 8) <- liftAction np_tx_fifo (@first SifiveUartFifoCapacity (Bit 8) ty) ;
-        Let hasData : Bool <- ##txHead `? "Some" ;
-        If #hasData Then (
-          Let txByte : Bit 8 <- ##txHead `! "Some" ;
-          Act (Send sifiveUartTxDataPath #txByte Retv) ;
-          Recv "txRdy" sifiveUartTxRdyPath (fun txRdy =>
-            If #txRdy Then (
-              Act (liftAction np_tx_fifo (@deq SifiveUartFifoCapacity (Bit 8) ty)) ;
-              Retv
-            ) ;
-            Retv
-          )
+    (* Read rxdata: dequeues byte from RX FIFO if available, bit 31 indicates empty *)
+    Definition readRxData : Action ty sifiveUartTree (Bit Xlen) :=
+      LetA rxEmpty : Bool <- liftAction np_rx_fifo (@isEmpty dom SifiveUartFifoCapacity (Bit 8) ty) ;
+      LetIf rxByte : Bit 8 <-
+        If (Not #rxEmpty) Then (
+          LetA rxHead : Option (Bit 8) <- liftAction np_rx_fifo (@first dom SifiveUartFifoCapacity (Bit 8) ty) ;
+          Act (liftAction np_rx_fifo (@deq dom SifiveUartFifoCapacity (Bit 8) ty)) ;
+          Return (##rxHead `! "Some")
+        ) Else (
+          Return $0
         ) ;
-        Retv
-      ) ;
-      Retv
-    ) ;
-    Retv.
+      Return {< ToBit #rxEmpty, Const ty (Bit (Xlen - 9)) Zmod.zero, #rxByte >}.
 
-  (* RX Rule: When rxen enabled and FIFO not full, sends rxRdy and samples rxData *)
-  Definition sifiveUartRxStep : Action ty sifiveUartTree (Bit 0) :=
-    LetA rxen : Bool <- ReadReg "rxctrl_rxen" sifiveUartRxctrlRxenPath (fun v => Return #v) ;
-    If #rxen Then (
-      LetA rxFull : Bool <- liftAction np_rx_fifo (@isFull SifiveUartFifoCapacity (Bit 8) ty) ;
-      If (Not #rxFull) Then (
-        Act (Send sifiveUartRxRdyPath (Const ty (Bit 0) Zmod.zero) Retv) ;
-        Retv
-      ) ;
-      Recv "rxData" sifiveUartRxDataPath (fun rxOpt =>
-        Let hasData : Bool <- ##rxOpt `? "Some" ;
-        If #hasData Then (
-          Let rxByte : Bit 8 <- ##rxOpt `! "Some" ;
-          If (Not #rxFull) Then (
-            Act (liftAction np_rx_fifo (@enq SifiveUartFifoCapacity (Bit 8) ty rxByte)) ;
-            Retv
+    (* Read ip: reads registered interrupt pending flags *)
+    Definition readIp : Action ty sifiveUartTree (Bit Xlen) :=
+      LetA txwm_ip : Bool <- ReadReg "ip_txwm" sifiveUartIpTxwmPath (fun v => Return #v) ;
+      LetA rxwm_ip : Bool <- ReadReg "ip_rxwm" sifiveUartIpRxwmPath (fun v => Return #v) ;
+      Return {< Const ty (Bit (Xlen - 2)) Zmod.zero, ToBit #rxwm_ip, ToBit #txwm_ip >}.
+
+    (* Autonomous rule to update ip_txwm and ip_rxwm registers *)
+    Definition sifiveUartIpStep : Action ty sifiveUartTree (Bit 0) :=
+      LetA txCount : Bit SifiveUartFifoCountWidth <- liftAction np_tx_fifo (@fifoCount dom SifiveUartFifoCapacity (Bit 8) ty) ;
+      LetA rxCount : Bit SifiveUartFifoCountWidth <- liftAction np_rx_fifo (@fifoCount dom SifiveUartFifoCapacity (Bit 8) ty) ;
+      LetA txcnt   : Bit SifiveUartWatermarkWidth <- ReadReg "txctrl_txcnt" sifiveUartTxctrlTxcntPath (fun v => Return #v) ;
+      LetA rxcnt   : Bit SifiveUartWatermarkWidth <- ReadReg "rxctrl_rxcnt" sifiveUartRxctrlRxcntPath (fun v => Return #v) ;
+      Let txwm_ip  : Bool <- Slt #txCount (ZeroExtendTo SifiveUartFifoCountWidth #txcnt) ;
+      Let rxwm_ip  : Bool <- Sgt #rxCount (ZeroExtendTo SifiveUartFifoCountWidth #rxcnt) ;
+      Act (WriteReg sifiveUartIpTxwmPath #txwm_ip Retv) ;
+      WriteReg sifiveUartIpRxwmPath #rxwm_ip Retv.
+
+    (* SiFive UART Interrupt Rule: writes interrupt status into cross register *)
+    Definition sifiveUartIrq : Action ty sifiveUartTree (Bit 0) :=
+      LetA txwm_ip : Bool <- ReadReg "ip_txwm" sifiveUartIpTxwmPath (fun v => Return #v) ;
+      LetA rxwm_ip : Bool <- ReadReg "ip_rxwm" sifiveUartIpRxwmPath (fun v => Return #v) ;
+      LetA ie_txwm : Bool <- ReadReg "ie_txwm" sifiveUartIeTxwmPath (fun v => Return #v) ;
+      LetA ie_rxwm : Bool <- ReadReg "ie_rxwm" sifiveUartIeRxwmPath (fun v => Return #v) ;
+      Let tx_irq   : Bool <- And [ #txwm_ip ; #ie_txwm ] ;
+      Let rx_irq   : Bool <- And [ #rxwm_ip ; #ie_rxwm ] ;
+      Let any_irq  : Bool <- Or [ #tx_irq ; #rx_irq ] ;
+      WriteReg sifiveUartIrqPath #any_irq Retv.
+
+    (* SiFive UART Interrupt Output: reads cross register for PLIC connection *)
+    Definition readSifiveUartIrq : Action ty sifiveUartTree Bool :=
+      ReadReg "irq" sifiveUartIrqPath (fun v => Return #v).
+
+    (* =========================================================================
+     * Decoupled Hardware Rules for Streaming PHY Interface & Divisor Export
+     * ========================================================================= *)
+
+    (* Autonomous rule to export divisor on divOut *)
+    Definition sifiveUartDivStep : Action ty sifiveUartTree (Bit 0) :=
+      ReadReg "div" sifiveUartDivPath (fun divVal =>
+        Send sifiveUartDivOutPath #divVal Retv
+      ).
+
+    (* TX Rule: When enabled and not empty, presents data on txData and dequeues on txRdy *)
+    Definition sifiveUartTxStep : Action ty sifiveUartTree (Bit 0) :=
+      LetA txen : Bool <- ReadReg "txctrl_txen" sifiveUartTxctrlTxenPath (fun v => Return #v) ;
+      If #txen Then (
+        LetA txEmpty : Bool <- liftAction np_tx_fifo (@isEmpty dom SifiveUartFifoCapacity (Bit 8) ty) ;
+        If (Not #txEmpty) Then (
+          LetA txHead : Option (Bit 8) <- liftAction np_tx_fifo (@first dom SifiveUartFifoCapacity (Bit 8) ty) ;
+          Let hasData : Bool <- ##txHead `? "Some" ;
+          If #hasData Then (
+            Let txByte : Bit 8 <- ##txHead `! "Some" ;
+            Act (Send sifiveUartTxDataPath #txByte Retv) ;
+            Recv "txRdy" sifiveUartTxRdyPath (fun txRdy =>
+              If #txRdy Then (
+                Act (liftAction np_tx_fifo (@deq dom SifiveUartFifoCapacity (Bit 8) ty)) ;
+                Retv
+              ) ;
+              Retv
+            )
           ) ;
           Retv
         ) ;
         Retv
-      )
+      ) ;
+      Retv.
+
+    (* RX Rule: When rxen enabled and FIFO not full, sends rxRdy and samples rxData *)
+    Definition sifiveUartRxStep : Action ty sifiveUartTree (Bit 0) :=
+      LetA rxen : Bool <- ReadReg "rxctrl_rxen" sifiveUartRxctrlRxenPath (fun v => Return #v) ;
+      If #rxen Then (
+        LetA rxFull : Bool <- liftAction np_rx_fifo (@isFull dom SifiveUartFifoCapacity (Bit 8) ty) ;
+        If (Not #rxFull) Then (
+          Act (Send sifiveUartRxRdyPath (Const ty (Bit 0) Zmod.zero) Retv) ;
+          Retv
+        ) ;
+        Recv "rxData" sifiveUartRxDataPath (fun rxOpt =>
+          Let hasData : Bool <- ##rxOpt `? "Some" ;
+          If #hasData Then (
+            Let rxByte : Bit 8 <- ##rxOpt `! "Some" ;
+            If (Not #rxFull) Then (
+              Act (liftAction np_rx_fifo (@enq dom SifiveUartFifoCapacity (Bit 8) ty rxByte)) ;
+              Retv
+            ) ;
+            Retv
+          ) ;
+          Retv
+        )
+      ) ;
+      Retv.
+
+  End SifiveUartOperations.
+
+  Arguments readTxData {ty}.
+  Arguments readRxData {ty}.
+  Arguments readIp {ty}.
+  Arguments sifiveUartIpStep {ty}.
+  Arguments sifiveUartIrq {ty}.
+  Arguments readSifiveUartIrq {ty}.
+  Arguments sifiveUartDivStep {ty}.
+  Arguments sifiveUartTxStep {ty}.
+  Arguments sifiveUartRxStep {ty}.
+  Arguments fifoCount {dom capacity k ty}.
+
+  (* ===========================================================================
+   * MMIO Line Read & Write Actions
+   * =========================================================================== *)
+
+  Definition sifiveUartLineReadAction
+             (base : Z)
+             (ty : Kind -> Type)
+             (addr : Expr ty Addr)
+             : Action ty sifiveUartTree (LineReadRp SifiveUartLineConfig) :=
+    Let offset <- getMemOffset base SifiveUartSizeBytes addr ;
+    Let regIdx : Bit SifiveUartRegIdxWidth <- TruncMsb SifiveUartRegIdxWidth LgNumBytesXlen #offset ;
+    Let isTxData : Bool <- Eq #regIdx (sifiveUartRegIdxBit "txdata") ;
+    Let isRxData : Bool <- Eq #regIdx (sifiveUartRegIdxBit "rxdata") ;
+    Let isTxCtrl : Bool <- Eq #regIdx (sifiveUartRegIdxBit "txctrl") ;
+    Let isRxCtrl : Bool <- Eq #regIdx (sifiveUartRegIdxBit "rxctrl") ;
+    Let isIe     : Bool <- Eq #regIdx (sifiveUartRegIdxBit "ie") ;
+    Let isIp     : Bool <- Eq #regIdx (sifiveUartRegIdxBit "ip") ;
+    Let isDiv    : Bool <- Eq #regIdx (sifiveUartRegIdxBit "div") ;
+    LetIf txDataWord : Bit Xlen <-
+      If #isTxData Then readTxData Else (Return $0) ;
+    LetIf rxDataWord : Bit Xlen <-
+      If #isRxData Then readRxData Else (Return $0) ;
+    LetIf ipWord : Bit Xlen <-
+      If #isIp Then readIp Else (Return $0) ;
+    ReadReg "txctrl_txen"  sifiveUartTxctrlTxenPath  (fun txen =>
+    ReadReg "txctrl_nstop" sifiveUartTxctrlNstopPath (fun nstop =>
+    ReadReg "txctrl_txcnt" sifiveUartTxctrlTxcntPath (fun txcnt =>
+    ReadReg "rxctrl_rxen"  sifiveUartRxctrlRxenPath  (fun rxen =>
+    ReadReg "rxctrl_rxcnt" sifiveUartRxctrlRxcntPath (fun rxcnt =>
+    ReadReg "ie_txwm"      sifiveUartIeTxwmPath      (fun ie_txwm =>
+    ReadReg "ie_rxwm"      sifiveUartIeRxwmPath      (fun ie_rxwm =>
+    ReadReg "div"          sifiveUartDivPath         (fun divVal =>
+    Let txctrlWord : Bit Xlen <-
+      {< Const ty (Bit (16 - SifiveUartWatermarkWidth)) Zmod.zero,
+         #txcnt,
+         Const ty (Bit 14) Zmod.zero,
+         ToBit #nstop,
+         ToBit #txen >} ;
+    Let rxctrlWord : Bit Xlen <-
+      {< Const ty (Bit (16 - SifiveUartWatermarkWidth)) Zmod.zero,
+         #rxcnt,
+         Const ty (Bit 15) Zmod.zero,
+         ToBit #rxen >} ;
+    Let ieWord : Bit Xlen <-
+      {< Const ty (Bit (Xlen - 2)) Zmod.zero,
+         ToBit #ie_rxwm,
+         ToBit #ie_txwm >} ;
+    Let divWord : Bit Xlen <-
+      {< Const ty (Bit (Xlen - 16)) Zmod.zero,
+         #divVal >} ;
+    Let readWord : Bit Xlen <-
+      Or [ ITE0 #isTxData #txDataWord ;
+           ITE0 #isRxData #rxDataWord ;
+           ITE0 #isTxCtrl #txctrlWord ;
+           ITE0 #isRxCtrl #rxctrlWord ;
+           ITE0 #isIe     #ieWord ;
+           ITE0 #isIp     #ipWord ;
+           ITE0 #isDiv    #divWord ] ;
+    Let dataArr : Array (cfgLineBytes SifiveUartLineConfig) (Bit 8) <-
+      FromBit (Array (cfgLineBytes SifiveUartLineConfig) (Bit 8)) #readWord ;
+    @Return ty sifiveUartTree (LineReadRp SifiveUartLineConfig) (STRUCT {
+      "data" ::= #dataArr ;
+      "tag"  ::= Const ty (Array (cfgNumLineTags SifiveUartLineConfig) Bool) (getDefault _)
+    }))))))))).
+
+  Definition sifiveUartLineWriteAction
+             (base : Z)
+             (ty : Kind -> Type)
+             (rq : Expr ty (LineWriteRq SifiveUartLineConfig))
+             : Action ty sifiveUartTree (Bit 0) :=
+    Let offset <- getMemOffset base SifiveUartSizeBytes (rq`"addr") ;
+    Let regIdx : Bit SifiveUartRegIdxWidth <- TruncMsb SifiveUartRegIdxWidth LgNumBytesXlen #offset ;
+    Let writeWord : Bit Xlen <- ToBit (rq`"data") ;
+    Let writeBits : Array (Z.to_nat Xlen) Bool <-
+      FromBit (Array (Z.to_nat Xlen) Bool) #writeWord ;
+    Let dataByte : Bit 8 <- TruncLsb (Xlen - 8) 8 #writeWord ;
+    If (Eq #regIdx (sifiveUartRegIdxBit "txdata")) Then (
+      LetA txFull : Bool <- liftAction np_tx_fifo (@isFull dom SifiveUartFifoCapacity (Bit 8) ty) ;
+      If (Not #txFull) Then (
+        liftAction np_tx_fifo (@enq dom SifiveUartFifoCapacity (Bit 8) ty dataByte)
+      ) ;
+      Retv
+    ) ;
+    If (Eq #regIdx (sifiveUartRegIdxBit "txctrl")) Then (
+      Act (WriteReg sifiveUartTxctrlTxenPath (##writeBits$[0]) Retv) ;
+      Act (WriteReg sifiveUartTxctrlNstopPath (##writeBits$[1]) Retv) ;
+      WriteReg sifiveUartTxctrlTxcntPath (TruncLsb (16 - SifiveUartWatermarkWidth) SifiveUartWatermarkWidth (TruncMsb 16 16 #writeWord)) Retv
+    ) ;
+    If (Eq #regIdx (sifiveUartRegIdxBit "rxctrl")) Then (
+      Act (WriteReg sifiveUartRxctrlRxenPath (##writeBits$[0]) Retv) ;
+      WriteReg sifiveUartRxctrlRxcntPath (TruncLsb (16 - SifiveUartWatermarkWidth) SifiveUartWatermarkWidth (TruncMsb 16 16 #writeWord)) Retv
+    ) ;
+    If (Eq #regIdx (sifiveUartRegIdxBit "ie")) Then (
+      Act (WriteReg sifiveUartIeTxwmPath (##writeBits$[0]) Retv) ;
+      WriteReg sifiveUartIeRxwmPath (##writeBits$[1]) Retv
+    ) ;
+    If (Eq #regIdx (sifiveUartRegIdxBit "div")) Then (
+      WriteReg sifiveUartDivPath (TruncLsb 16 16 #writeWord) Retv
     ) ;
     Retv.
 
-End SifiveUartOperations.
+  (* ===========================================================================
+   * MemRegion Constructor
+   * =========================================================================== *)
 
-Arguments readTxData {ty}.
-Arguments readRxData {ty}.
-Arguments readIp {ty}.
-Arguments sifiveUartIpStep {ty}.
-Arguments sifiveUartIrq {ty}.
-Arguments sifiveUartDivStep {ty}.
-Arguments sifiveUartTxStep {ty}.
-Arguments sifiveUartRxStep {ty}.
-Arguments fifoCount {capacity k ty}.
+  Definition sifiveUartMemRegion
+             (base : Z)
+             (pfBound : Is_true ((0 <=? base) && (base + SifiveUartSizeBytes <=? Z.shiftl 1 AddrSz))%Z)
+             (pfAligned : Is_true (base mod (2 ^ Z.of_nat (cfgLgLineBytes SifiveUartLineConfig)) =? 0)%Z)
+             : MemRegion := {|
+    regionName        := "sifive_uart" ;
+    regionDom         := dom ;
+    regionBase        := base ;
+    regionSize        := SifiveUartSizeBytes ;
+    regionLineCfg     := SifiveUartLineConfig ;
+    isReadOnly        := false ;
+    regionKind        := @CustomMem "sifive_uart" SifiveUartSizeBytes SifiveUartLineConfig
+                                    sifiveUartChildren
+                                    (sifiveUartLineReadAction base)
+                                    (sifiveUartLineWriteAction base)
+                                    (Some (fun ty => readSifiveUartIrq (ty:=ty))) ;
+    regionInMemory    := pfBound ;
+    regionBaseAligned := pfAligned ;
+    regionSizeAligned := I
+  |}.
 
-(* ===========================================================================
- * MMIO Line Read & Write Actions
- * =========================================================================== *)
+  Arguments sifiveUartMemRegion base pfBound pfAligned : clear implicits.
 
-Definition sifiveUartLineReadAction
-           (base : Z)
-           (ty : Kind -> Type)
-           (addr : Expr ty Addr)
-           : Action ty sifiveUartTree (LineReadRp SifiveUartLineConfig) :=
-  Let offset <- getMemOffset base SifiveUartSizeBytes addr ;
-  Let regIdx : Bit SifiveUartRegIdxWidth <- TruncMsb SifiveUartRegIdxWidth LgNumBytesXlen #offset ;
-  Let isTxData : Bool <- Eq #regIdx (sifiveUartRegIdxBit "txdata") ;
-  Let isRxData : Bool <- Eq #regIdx (sifiveUartRegIdxBit "rxdata") ;
-  Let isTxCtrl : Bool <- Eq #regIdx (sifiveUartRegIdxBit "txctrl") ;
-  Let isRxCtrl : Bool <- Eq #regIdx (sifiveUartRegIdxBit "rxctrl") ;
-  Let isIe     : Bool <- Eq #regIdx (sifiveUartRegIdxBit "ie") ;
-  Let isIp     : Bool <- Eq #regIdx (sifiveUartRegIdxBit "ip") ;
-  Let isDiv    : Bool <- Eq #regIdx (sifiveUartRegIdxBit "div") ;
-  LetIf txDataWord : Bit Xlen <-
-    If #isTxData Then readTxData Else (Return $0) ;
-  LetIf rxDataWord : Bit Xlen <-
-    If #isRxData Then readRxData Else (Return $0) ;
-  LetIf ipWord : Bit Xlen <-
-    If #isIp Then readIp Else (Return $0) ;
-  ReadReg "txctrl_txen"  sifiveUartTxctrlTxenPath  (fun txen =>
-  ReadReg "txctrl_nstop" sifiveUartTxctrlNstopPath (fun nstop =>
-  ReadReg "txctrl_txcnt" sifiveUartTxctrlTxcntPath (fun txcnt =>
-  ReadReg "rxctrl_rxen"  sifiveUartRxctrlRxenPath  (fun rxen =>
-  ReadReg "rxctrl_rxcnt" sifiveUartRxctrlRxcntPath (fun rxcnt =>
-  ReadReg "ie_txwm"      sifiveUartIeTxwmPath      (fun ie_txwm =>
-  ReadReg "ie_rxwm"      sifiveUartIeRxwmPath      (fun ie_rxwm =>
-  ReadReg "div"          sifiveUartDivPath         (fun divVal =>
-  Let txctrlWord : Bit Xlen <-
-    {< Const ty (Bit (16 - SifiveUartWatermarkWidth)) Zmod.zero,
-       #txcnt,
-       Const ty (Bit 14) Zmod.zero,
-       ToBit #nstop,
-       ToBit #txen >} ;
-  Let rxctrlWord : Bit Xlen <-
-    {< Const ty (Bit (16 - SifiveUartWatermarkWidth)) Zmod.zero,
-       #rxcnt,
-       Const ty (Bit 15) Zmod.zero,
-       ToBit #rxen >} ;
-  Let ieWord : Bit Xlen <-
-    {< Const ty (Bit (Xlen - 2)) Zmod.zero,
-       ToBit #ie_rxwm,
-       ToBit #ie_txwm >} ;
-  Let divWord : Bit Xlen <-
-    {< Const ty (Bit (Xlen - 16)) Zmod.zero,
-       #divVal >} ;
-  Let readWord : Bit Xlen <-
-    Or [ ITE0 #isTxData #txDataWord ;
-         ITE0 #isRxData #rxDataWord ;
-         ITE0 #isTxCtrl #txctrlWord ;
-         ITE0 #isRxCtrl #rxctrlWord ;
-         ITE0 #isIe     #ieWord ;
-         ITE0 #isIp     #ipWord ;
-         ITE0 #isDiv    #divWord ] ;
-  Let dataArr : Array (cfgLineBytes SifiveUartLineConfig) (Bit 8) <-
-    FromBit (Array (cfgLineBytes SifiveUartLineConfig) (Bit 8)) #readWord ;
-  @Return ty sifiveUartTree (LineReadRp SifiveUartLineConfig) (STRUCT {
-    "data" ::= #dataArr ;
-    "tag"  ::= Const ty (Array (cfgNumLineTags SifiveUartLineConfig) Bool) (getDefault _)
-  }))))))))).
+  (* ===========================================================================
+   * System Integration Helpers
+   * =========================================================================== *)
 
-Definition sifiveUartLineWriteAction
-           (base : Z)
-           (ty : Kind -> Type)
-           (rq : Expr ty (LineWriteRq SifiveUartLineConfig))
-           : Action ty sifiveUartTree (Bit 0) :=
-  Let offset <- getMemOffset base SifiveUartSizeBytes (rq`"addr") ;
-  Let regIdx : Bit SifiveUartRegIdxWidth <- TruncMsb SifiveUartRegIdxWidth LgNumBytesXlen #offset ;
-  Let writeWord : Bit Xlen <- ToBit (rq`"data") ;
-  Let writeBits : Array (Z.to_nat Xlen) Bool <-
-    FromBit (Array (Z.to_nat Xlen) Bool) #writeWord ;
-  Let dataByte : Bit 8 <- TruncLsb (Xlen - 8) 8 #writeWord ;
-  If (Eq #regIdx (sifiveUartRegIdxBit "txdata")) Then (
-    LetA txFull : Bool <- liftAction np_tx_fifo (@isFull SifiveUartFifoCapacity (Bit 8) ty) ;
-    If (Not #txFull) Then (
-      liftAction np_tx_fifo (@enq SifiveUartFifoCapacity (Bit 8) ty dataByte)
-    ) ;
-    Retv
-  ) ;
-  If (Eq #regIdx (sifiveUartRegIdxBit "txctrl")) Then (
-    Act (WriteReg sifiveUartTxctrlTxenPath (##writeBits$[0]) Retv) ;
-    Act (WriteReg sifiveUartTxctrlNstopPath (##writeBits$[1]) Retv) ;
-    WriteReg sifiveUartTxctrlTxcntPath (TruncLsb (16 - SifiveUartWatermarkWidth) SifiveUartWatermarkWidth (TruncMsb 16 16 #writeWord)) Retv
-  ) ;
-  If (Eq #regIdx (sifiveUartRegIdxBit "rxctrl")) Then (
-    Act (WriteReg sifiveUartRxctrlRxenPath (##writeBits$[0]) Retv) ;
-    WriteReg sifiveUartRxctrlRxcntPath (TruncLsb (16 - SifiveUartWatermarkWidth) SifiveUartWatermarkWidth (TruncMsb 16 16 #writeWord)) Retv
-  ) ;
-  If (Eq #regIdx (sifiveUartRegIdxBit "ie")) Then (
-    Act (WriteReg sifiveUartIeTxwmPath (##writeBits$[0]) Retv) ;
-    WriteReg sifiveUartIeRxwmPath (##writeBits$[1]) Retv
-  ) ;
-  If (Eq #regIdx (sifiveUartRegIdxBit "div")) Then (
-    WriteReg sifiveUartDivPath (TruncLsb 16 16 #writeWord) Retv
-  ) ;
-  Retv.
+  Record SifiveUartInstance (regions : list MemRegion) := {
+    sifiveUartIdx      : nat ;
+    sifiveUartBaseAddr : Z ;
+    pfBound            : Is_true ((0 <=? sifiveUartBaseAddr) && (sifiveUartBaseAddr + SifiveUartSizeBytes <=? Z.shiftl 1 AddrSz))%Z ;
+    pfAligned          : Is_true (sifiveUartBaseAddr mod (2 ^ Z.of_nat (cfgLgLineBytes SifiveUartLineConfig)) =? 0)%Z ;
+    pfSifiveUart       : nth_error regions sifiveUartIdx = Some (sifiveUartMemRegion sifiveUartBaseAddr pfBound pfAligned)
+  }.
 
-Arguments sifiveUartLineReadAction base ty addr : clear implicits.
-Arguments sifiveUartLineWriteAction base ty rq : clear implicits.
+  Definition sifiveUartRegion {regions} (uart : SifiveUartInstance regions) : MemRegion :=
+    sifiveUartMemRegion uart.(sifiveUartBaseAddr) uart.(pfBound) uart.(pfAligned).
 
-(* ===========================================================================
- * MemRegion Constructor
- * =========================================================================== *)
+  Section SifiveUartSystem.
+    Variable regions : list MemRegion.
+    Variable uart : SifiveUartInstance regions.
+    Variable ty : Kind -> Type.
 
-Definition sifiveUartMemRegion
-           (base : Z)
-           (pfBound : Is_true ((0 <=? base) && (base + SifiveUartSizeBytes <=? Z.shiftl 1 AddrSz))%Z)
-           (pfAligned : Is_true (base mod (2 ^ Z.of_nat (cfgLgLineBytes SifiveUartLineConfig)) =? 0)%Z)
-           : MemRegion := {|
-  regionName        := "sifive_uart" ;
-  regionBase        := base ;
-  regionSize        := SifiveUartSizeBytes ;
-  regionLineCfg     := SifiveUartLineConfig ;
-  isReadOnly        := false ;
-  regionKind        := @CustomMem "sifive_uart" SifiveUartSizeBytes SifiveUartLineConfig
-                                  sifiveUartChildren
-                                  (sifiveUartLineReadAction base)
-                                  (sifiveUartLineWriteAction base)
-                                  (Some (fun ty => sifiveUartIrq (ty:=ty))) ;
-  regionInMemory    := pfBound ;
-  regionBaseAligned := pfAligned ;
-  regionSizeAligned := I
-|}.
+    Local Notation memTree := (specMemTree regions).
 
-Arguments sifiveUartMemRegion base pfBound pfAligned : clear implicits.
+    Definition sifiveUartAction {k : Kind} (act : Action ty sifiveUartTree k) : Action ty memTree k :=
+      nthRegionAction uart.(sifiveUartIdx) regions (sifiveUartRegion uart) uart.(pfSifiveUart) act.
 
-(* ===========================================================================
- * System Integration Helpers
- * =========================================================================== *)
+    Definition sifiveUartIpStepAction : Action ty memTree (Bit 0) :=
+      sifiveUartAction (@sifiveUartIpStep ty).
 
-Record SifiveUartInstance (regions : list MemRegion) := {
-  sifiveUartIdx      : nat ;
-  sifiveUartBaseAddr : Z ;
-  pfBound            : Is_true ((0 <=? sifiveUartBaseAddr) && (sifiveUartBaseAddr + SifiveUartSizeBytes <=? Z.shiftl 1 AddrSz))%Z ;
-  pfAligned          : Is_true (sifiveUartBaseAddr mod (2 ^ Z.of_nat (cfgLgLineBytes SifiveUartLineConfig)) =? 0)%Z ;
-  pfSifiveUart       : nth_error regions sifiveUartIdx = Some (sifiveUartMemRegion sifiveUartBaseAddr pfBound pfAligned)
-}.
+    Definition sifiveUartIrqStepAction : Action ty memTree (Bit 0) :=
+      sifiveUartAction (@sifiveUartIrq ty).
 
-Definition sifiveUartRegion {regions} (uart : SifiveUartInstance regions) : MemRegion :=
-  sifiveUartMemRegion uart.(sifiveUartBaseAddr) uart.(pfBound) uart.(pfAligned).
+    Definition sifiveUartDivStepAction : Action ty memTree (Bit 0) :=
+      sifiveUartAction (@sifiveUartDivStep ty).
 
-Section SifiveUartSystem.
-  Variable regions : list MemRegion.
-  Variable uart : SifiveUartInstance regions.
-  Variable ty : Kind -> Type.
+    Definition sifiveUartTxStepAction : Action ty memTree (Bit 0) :=
+      sifiveUartAction (@sifiveUartTxStep ty).
 
-  Local Notation memTree := (specMemTree regions).
+    Definition sifiveUartRxStepAction : Action ty memTree (Bit 0) :=
+      sifiveUartAction (@sifiveUartRxStep ty).
 
-  Definition sifiveUartAction {k : Kind} (act : Action ty sifiveUartTree k) : Action ty memTree k :=
-    nthRegionAction uart.(sifiveUartIdx) regions (sifiveUartRegion uart) uart.(pfSifiveUart) act.
+  End SifiveUartSystem.
 
-  Definition sifiveUartIpStepAction : Action ty memTree (Bit 0) :=
-    sifiveUartAction (@sifiveUartIpStep ty).
-
-  Definition sifiveUartDivStepAction : Action ty memTree (Bit 0) :=
-    sifiveUartAction (@sifiveUartDivStep ty).
-
-  Definition sifiveUartTxStepAction : Action ty memTree (Bit 0) :=
-    sifiveUartAction (@sifiveUartTxStep ty).
-
-  Definition sifiveUartRxStepAction : Action ty memTree (Bit 0) :=
-    sifiveUartAction (@sifiveUartRxStep ty).
-
-End SifiveUartSystem.
+End SifiveUart.
